Set up function

SSA/Experimental/Bits/Fast/Reflect.lean
@@ -17,9 +17,11 @@ import SSA.Experimental.Bits.Fast.Defs
 import SSA.Experimental.Bits.Fast.FiniteStateMachine
 import SSA.Experimental.Bits.Fast.Attr
 import SSA.Experimental.Bits.Fast.Decide
+import Std.Sat.AIG.CNF
+import Std.Sat.AIG.RelabelNat
+import Std.Tactic.BVDecide.Bitblast.BVExpr
 import Lean.Meta.ForEachExpr
 import Lean.Meta.Tactic.Simp.BuiltinSimprocs.BitVec
-
 import Lean
 
 /-
@@ -1558,6 +1560,82 @@ def checkCircuitSatAux [DecidableEq α] [Hashable α] [Fintype α] (c : Circuit 
     match out with
     | .error _model => return true
     | .ok _cert => return false
+
+
+
+open Std.Sat
+open Std.Tactic.BVDecide
+/--
+Verify that a proof certificate is valid for a given formula.
+-/
+def verifyCert (cnf : CNF Nat) (cert : String) : Bool :=
+  match LRAT.parseLRATProof cert.toUTF8 with
+  | .ok lratProof => LRAT.check lratProof cnf
+  | .error _ => false
+
+theorem verifyCert_correct : ∀ cnf cert, verifyCert cnf cert = true → cnf.Unsat := by
+  intro c b h1
+  unfold verifyCert at h1
+  split at h1
+  . apply LRAT.check_sound
+    assumption
+  . contradiction
+
+/--
+Verify that `cert` is an UNSAT proof for the SAT problem obtained by bitblasting `bv`.
+-/
+def verifyBVExpr (bv : BVLogicalExpr) (cert : String) : Bool :=
+  verifyCert (AIG.toCNF bv.bitblast.relabelNat) cert
+
+theorem unsat_of_verifyBVExpr_eq_true (bv : BVLogicalExpr) (c : String)
+    (h : verifyBVExpr bv c = true) :
+    bv.Unsat := by
+  apply BVLogicalExpr.unsat_of_bitblast
+  rw [← AIG.Entrypoint.relabelNat_unsat_iff]
+  rw [← AIG.toCNF_equisat]
+  apply verifyCert_correct
+  rw [verifyBVExpr] at h
+  assumption
+
+open Std Sat AIG Tactic BVDecide Frontend in
+def solver (bvExpr: BVLogicalExpr) : TermElabM (Except (Array (Bool × Nat)) UnsatProver.Result) := do
+    let cfg: BVDecideConfig := {timeout := 10}
+    IO.FS.withTempFile fun _ lratFile => do
+      let ctx ← BVDecide.Frontend.TacticContext.new lratFile cfg
+      logInfo m! "Bitblasting BVLogicalExpr to AIG"
+      let entry ← IO.lazyPure (fun _ => bvExpr.bitblast)
+
+      logInfo m! "Converting AIG to CNF"
+      let (cnf, map) ← IO.lazyPure (fun _ =>
+            let (entry, map) := entry.relabelNat' -- [TODO: Why do we have the prime?]
+            let cnf := AIG.toCNF entry
+            (cnf, map))
+
+      logInfo m! "Obtaining external proof certificate"
+      let res ← runExternal cnf ctx.solver ctx.lratPath
+          (trimProofs := true)
+          (timeout := cadicalTimeoutSec)
+          (binaryProofs := true)
+
+      match res with
+      | .ok cert =>
+        logInfo m! "SAT solver found a proof."
+        let proof ← cert.toReflectionProof ctx bvExpr ``verifyBVExpr ``unsat_of_verifyBVExpr_eq_true
+        return .ok ⟨proof, cert⟩
+      | .error assignment =>
+        logInfo m! "SAT solver found a counter example."
+        -- let equations := reconstructCounterExample map assignment entry.aig.decls.size atomsAssignment
+        return .error assignment
+
+def bvExpr : BVLogicalExpr :=
+  let x := BVExpr.const (BitVec.ofNat 64 2)
+  let y := BVExpr.const (BitVec.ofNat 64 4)
+  let z := BVExpr.const (BitVec.ofNat 64 8)
+  let sum := BVExpr.bin x BVBinOp.add y
+  BoolExpr.literal (BVPred.bin sum BVBinPred.eq z)
+
+--- need to create a toString
+#eval solver bvExpr
 
 
 open Std Sat AIG Tactic BVDecide Frontend in
